Test/test.lean
@@ -1,0 +1,103 @@
+import Plausible
+
+import Std.Data.HashMap
+open Std
+
+set_option maxHeartbeats 0
+
+
+def swapFirstAndLast_precond (a : Array Int) : Prop :=
+  a.size > 0
+
+def swapFirstAndLast (a : Array Int) (h_precond: swapFirstAndLast_precond a) : Array Int :=
+  let first := a[0]!
+  let last := a[a.size - 1]!
+  a.set! 0 last |>.set! (a.size - 1) first
+
+@[reducible, simp]
+def swapFirstAndLast_postcond (a : Array Int) (result : Array Int) (h_precond: swapFirstAndLast_precond a) : Prop :=
+  result.size = a.size ∧
+  result[0]! = a[a.size - 1]! ∧
+  result[result.size - 1]! = a[0]! ∧
+  (List.range (result.size - 2)).all (fun i => result[i + 1]! = a[i + 1]!)
+
+namespace test1
+
+@[reducible]
+def majorityElement_precond (nums : List Int) : Prop :=
+  nums.length > 0 ∧ nums.any (fun x => nums.count x > nums.length / 2)
+
+def majorityElement (nums : List Int) (h_precond : majorityElement_precond (nums)) : Int :=
+  Id.run do
+    let mut counts : HashMap Int Nat := {}
+    let n := nums.length
+    for x in nums do
+      let count := counts.getD x 0
+      counts := counts.insert x (count + 1)
+    match counts.toList.find? (fun (_, c) => c > n / 2) with
+    | some (k, _) => k
+    | none      => 0
+
+@[reducible]
+def majorityElement_postcond (nums : List Int) (result: Int) (h_precond : majorityElement_precond (nums)) : Prop :=
+  let n := nums.length
+  (nums.count result) > n / 2
+  ∧ ∀ x, x ≠ result → nums.count x ≤ n / 2
+
+theorem majorityElement_spec_satisfied (nums: List Int) (h_precond : majorityElement_precond (nums)) :
+    majorityElement_postcond (nums) (majorityElement (nums) h_precond) h_precond := by
+    dsimp [majorityElement_postcond, majorityElement]
+    plausible (config := { numInst := 1000, maxSize := 100, numRetries := 20, randomSeed := some 42})
+
+end test1
+
+
+namespace test2
+
+def listToNat : List Nat → Nat
+| []       => 0
+| d :: ds  => d + 10 * listToNat ds
+
+@[reducible]
+def addTwoNumbers_precond (l1 : List Nat) (l2 : List Nat) : Prop :=
+  l1.length > 0 ∧ l2.length > 0
+  ∧ (∀ d ∈ l1, d < 10) ∧ (∀ d ∈ l2, d < 10)
+  ∧ (l1.getLast! ≠ 0 ∨ l1 = [0])
+  ∧ (l2.getLast! ≠ 0 ∨ l2 = [0])
+
+def addTwoNumbers (l1 : List Nat) (l2 : List Nat) (h_precond : addTwoNumbers_precond (l1) (l2)) : List Nat :=
+  let rec addAux (l1 l2 : List Nat) (carry : Nat) : List Nat :=
+    match l1, l2 with
+    | [], [] =>
+      if carry = 0 then [] else [carry]
+    | h1::t1, [] =>
+      let sum := h1 + carry
+      (sum % 10) :: addAux t1 [] (sum / 10)
+    | [], h2::t2 =>
+      let sum := h2 + carry
+      (sum % 10) :: addAux [] t2 (sum / 10)
+    | h1::t1, h2::t2 =>
+      let sum := h1 + h2 + carry
+      (sum % 10) :: addAux t1 t2 (sum / 10)
+  addAux l1 l2 0
+
+@[reducible]
+def addTwoNumbers_postcond (l1 : List Nat) (l2 : List Nat) (result: List Nat) (h_precond : addTwoNumbers_precond (l1) (l2)) : Prop :=
+  listToNat result = listToNat l1 + listToNat l2
+  ∧
+  (∀ d ∈ result, d < 10) ∧
+  (result.getLast! ≠ 0 ∨ (l1 = [0] ∧ l2 = [0] ∧ result = [0]))
+
+theorem addTwoNumbers_spec_satisfied (l1: List Nat) (l2: List Nat) (h_precond : addTwoNumbers_precond (l1) (l2)) :
+    addTwoNumbers_postcond (l1) (l2) (addTwoNumbers (l1) (l2) h_precond) h_precond := by
+    unfold addTwoNumbers addTwoNumbers_postcond
+    unfold addTwoNumbers_precond at h_precond
+    plausible (config := { numInst := 1000, maxSize := 100, numRetries := 20, randomSeed := some 42})
+
+end test2
+
+
+/-- error: Found a counter-example! -/
+#guard_msgs in
+theorem type_u (α : Type u) (l : List α) : l = l ++ l := by
+  plausible (config := {quiet := true})
